Basically (?) finish grackle generation calendar example

testdata/out/coq/calendar_proof_gk.v
@@ -31,68 +31,75 @@ Definition has_encoding (encoded:list u8) (args:C) : Prop :=
   encoded = (u64_le $ length $ args.(hash')) ++ args.(hash') ++
               (u64_le $ length $ args.(events')) ++ events_enc
   /\ length args.(hash') < 2^64
+  /\ encodes events_enc args.(events') Event_gk.has_encoding
   /\ length args.(events') < 2^64.
 
 Definition own (args__v: calendar_gk.S.t) (args__c: C) (dq: dfrac) : iProp Σ :=
   ∃ (l__events : list event_gk.S.t), 
   "Hown_hash" ∷ own_slice args__v.(calendar_gk.S.Hash') dq args__c.(hash') ∗
-  "Hown_events_sl" ∷ own_slice args__v.(calendar_gk.S.Events') dq args__c.(events') ∗
-  "Hown_events_own" ∷ ([∗ list] x;c ∈ l__events;args__c.(events'), Event_gk.own x c dq).
+  "%Hown_hash_len" ∷ ⌜ length args__c.(hash') < 2^64 ⌝ ∗
+  "Hown_events_sl" ∷ own_slice args__v.(calendar_gk.S.Events') dq l__events ∗
+  "Hown_events_own" ∷ ([∗ list] x;c ∈ l__events;args__c.(events'), Event_gk.own x c dq) ∗
+  "%Hown_events_len" ∷ ⌜ length l__events < 2^64 ⌝.
 
-Lemma wp_Encode (args__c : calendar_gk.S.t) (pre_sl : slice.t) (prefix : list u8) (dq : dfrac):
-  length args__c.(calendar_gk.S.Hash') < 2^64 ->
+Lemma wp_Encode (args__t : calendar_gk.S.t) (args__c : C) (pre_sl : slice.t) (prefix : list u8) (dq : dfrac):
   {{{
         is_pkg_init calendar_gk ∗
+        own args__t args__c dq ∗ 
         own_slice pre_sl (DfracOwn 1) prefix ∗
         own_slice_cap w8 pre_sl
   }}}
-    calendar_gk @ "Marshal" #pre_sl #args__c
+    calendar_gk @ "Marshal" #pre_sl #args__t
   {{{
         enc enc_sl, RET #enc_sl;
         ⌜ has_encoding enc args__c ⌝ ∗
+        own args__t args__c dq ∗ 
         own_slice enc_sl (DfracOwn 1) (prefix ++ enc) ∗
         own_slice_cap w8 enc_sl
   }}}.
 
 Proof.
-  intros Hhashlen.
-  wp_start as "[Hsl Hcap]". wp_auto.
+  wp_start as "(Hown & Hsl & Hcap)". iNamed "Hown". wp_auto.
 
-  iDestruct (own_slice_small_sz with "Hown_hash") as "%Hargs_hash_sz".
-  wp_pures. wp_apply (wp_slice_len). wp_load.
-  wp_apply (wp_WriteInt with "[$Hsl]"). iIntros (?) "Hsl". wp_store.
-  wp_pures. wp_load.
-  wp_apply (wp_WriteBytes with "[$Hsl $Hown_hash]").
-  iIntros (?) "[Hsl Hargs_hash_sl]". wp_store.
+  iDestruct (own_slice_len with "Hown_hash") as "%Hown_hash_sz".
+  wp_apply (wp_WriteInt with "[$Hsl $Hcap]"). iIntros (?) "[Hsl Hcap]". wp_auto.
+  wp_apply (wp_WriteBytes with "[$Hsl $Hcap $Hown_hash]").
+  iIntros (?) "(Hsl & Hcap & Hown_hash)". wp_auto.
 
-  wp_apply (wp_slice_len).
-  wp_load. wp_apply (wp_WriteInt with "[$Hsl]").
-  iIntros (?) "Hsl". wp_store. wp_pures.
+  wp_apply (wp_WriteInt with "[$Hsl $Hcap]").
+  iIntros (?) "[Hsl Hcap]". wp_auto.
 
-  wp_load.
-  wp_apply (wp_WriteSlice _ _ args__c.(events) Event.has_encoding Event.own with "[Hown_events Hsl]").
+  iDestruct (own_slice_len with "Hown_events_sl") as "%Hown_events_sz".
+  iDestruct (big_sepL2_length with "Hown_events_own") as "%Hown_events_sz'".
+  rewrite Hown_events_sz' in Hown_events_sz.
+  wp_apply (wp_WriteSlice with "[$Hsl $Hown_events_sl $Hown_events_own]").
   {
-    iFrame.
     iIntros (????) "!>".
-    iIntros (?) "[Hown' Hsl'] HΦ".
-    wp_apply (Event.wp_Encode with "[$Hsl' $Hown']").
+    iIntros (?) "(Hown & Hsl & Hcap) HΦ".
+    wp_apply (Event_gk.wp_Encode with "[$Hown $Hsl $Hcap]").
     iApply "HΦ".
   }
-  iIntros (events_enc events_sl') "(Hpsl_events & %Henc_events & Hsl)".
-  wp_pures. wp_store.
-
+  iIntros (events_enc events_sl') "(Hown_events & Hown_events_own & %Henc_events & Hsl)".
+  wp_auto.
 
   iApply "HΦ". rewrite -?app_assoc.
   iFrame. iPureIntro.
 
   unfold has_encoding.
-  exists events_enc. 
-  split; first reflexivity.
-  repeat split.
-  all: word || done.
+  split; last done.
+  exists events_enc.
+  split.
+  {
+     rewrite Hown_hash_sz.
+     rewrite Hown_events_sz.
+     rewrite ?w64_to_nat_id.
+     congruence.
+  }
+  rewrite <- Hown_events_sz'.
+  done. 
 Qed.
 
-Lemma wp_Decode (enc : list u8) (enc_sl : slice.t) (args__c : calendar_gk.S.t) (suffix : list u8) (dq : dfrac):
+Lemma wp_Decode (enc : list u8) (enc_sl : slice.t) (args__c : C) (suffix : list u8) (dq : dfrac):
   {{{
         is_pkg_init calendar_gk ∗
         ⌜ has_encoding enc args__c ⌝ ∗
@@ -100,60 +107,34 @@ Lemma wp_Decode (enc : list u8) (enc_sl : slice.t) (args__c : calendar_gk.S.t) (
   }}}
     calendar_gk @ "Unmarshal" #enc_sl
   {{{
-        suff_sl, RET (#args__c, #suff_sl);
+        args__t suff_sl, RET (#args__t, #suff_sl);
+        own args__t args__c (DfracOwn 1) ∗ 
         own_slice suff_sl dq suffix
   }}}.
 
 Proof.
   wp_start as "[%Henc Hsl]". wp_auto.
   unfold has_encoding in Henc.
-  destruct Henc as ( events_enc & Henc & Henc_events & Hevents_sz ).
+  destruct Henc as ( events_enc & Henc & Hlen_hash & Henc_events & Hevents_sz ).
   rewrite Henc. rewrite -?app_assoc.
 
-  wp_apply wp_allocN; first done; first by val_ty.
-  iIntros (?) "HhashLen". iApply array_singleton in "HhashLen". wp_pures.
-  wp_apply wp_allocN; first done; first by val_ty.
-  iIntros (?) "HhashBytes". iApply array_singleton in "HhashBytes". wp_pures.
-  wp_load. wp_apply (wp_ReadInt with "[$Hsl]").
-  iIntros (?) "Hsl". wp_pures. wp_store. wp_store. wp_load. wp_load.
+  wp_apply (wp_ReadLenPrefixedBytes with "[$Hsl]"); first word.
+  iIntros (??) "[Hown_hash Hsl]". wp_auto.
 
-  iDestruct (own_slice_small_sz with "Hsl") as %Hhash_sz.
-  wp_apply (wp_ReadBytesCopy with "[$]").
-  { rewrite length_app in Hhash_sz. word. }
-  iIntros (??) "[Hhash' Hsl]". iApply own_slice_to_small in "Hhash'".
-
-  wp_pures. wp_store. wp_store. wp_load. wp_store.
-
-  wp_apply wp_ref_of_zero; first done.
-  iIntros (l__eventsLen) "HeventsLen". wp_pures.
-
-  wp_load. wp_apply (wp_ReadInt with "[Hsl]"); first simpl; iFrame.
-  iIntros (?) "Hsl". wp_pures. wp_store. wp_store.
-
-  wp_load. wp_load.
-  wp_apply (wp_ReadSlice _ _ _ _ Event.has_encoding Event.own with "[Hsl]").
+  wp_apply (wp_ReadInt with "[$Hsl]"). iIntros (?) "Hsl". wp_auto.
+  wp_apply (wp_ReadSlice with "[$Hsl]").
   {
-    iIntros (???) "Hown'".
-    iApply Event.own_val_ty.
-    iFrame.
-  } { done. }
-  {
-    iFrame.
-    iSplit; first done.
+    iSplit; auto.
     iSplit; first word.
     iIntros (????) "!>".
-    iIntros (?) "[Hsl' Henc'] HΦ".
-    wp_apply (Event.wp_Decode with "[$Hsl' $Henc']").
+    iIntros (?) "[Hsl Henc] HΦ".
+    wp_apply (Event_gk.wp_Decode with "[$Hsl $Henc]").
     iApply "HΦ".
   }
-  iIntros (??) "[Hpsl_events Hsl]".
-  wp_pures. wp_store. wp_store.
+  iIntros (???) "(Hown_events_sl & Hown_events_own & Hsl)". wp_auto.
 
-  replace {|
-    calendar_gk.S.Hash' := args__c.(calendar_gk.S.Hash');
-    calendar_gk.S.Events' := args__c.(calendar_gk.S.Events')
-  |} with args__c; last (destruct args__c; reflexivity).
   iApply "HΦ". iFrame.
+  done.
 Qed.
 
 End calendar_gk.
